fsub/lngen/prop_typing.v
@@ -13,6 +13,39 @@ Require Import fsub.lngen.def_extra.
 Require Import fsub.lngen.prop_basic.
 Require Import fsub.lngen.prop_subtyping.
 
+Lemma typing_subst_tvar Γ1 Γ2 X t A B C :
+  (Γ2 ++ (X, entry_tvar B) :: Γ1) ⊢ t : A ->
+  ⊢ (Γ2 ++ (X, entry_tvar B) :: Γ1) ->
+  Γ1 ⊢ C <: B ->
+  ((map (subst_typ_in_entry C X) Γ2) ++ Γ1) ⊢ subst_typ_in_exp C X t : subst_typ_in_typ C X A.
+Proof.
+  intros. dependent induction H; simpl; eauto using typing.
+  - econstructor.
+    + hauto use:subst_typ_in_typ_lc_typ, subtyping_wf_typ, wf_typ_lc_typ.
+    + admit.
+  - inst_cofinites_for typing_abs. 
+    + eapply wf_typ_subst_tvar; eauto.
+    + intros. inst_cofinites_with x.
+      rewrite_env ((map (subst_typ_in_entry C X) ((x, entry_var A) :: Γ2)) ++ Γ1).
+      setoid_rewrite subst_typ_in_exp_open_exp_wrt_exp in H1; try hauto use:subtyping_wf_typ.
+      move : H1 => /(_ _ _ X) H1. simpl in H1. destruct_eq_atom.
+      eapply H1; simpl; eauto.
+      eapply wf_cons_var; eauto.
+  - inst_cofinites_for typing_tabs.
+    + eapply wf_typ_subst_tvar; eauto.
+    + intros. inst_cofinites_with X0.
+      rewrite_env (map (subst_typ_in_entry C X) ((X0, entry_tvar A) :: Γ2) ++ Γ1).
+      setoid_rewrite subst_typ_in_typ_open_typ_wrt_typ in H1; try hauto use:subtyping_wf_typ.
+      setoid_rewrite subst_typ_in_exp_open_exp_wrt_typ in H1; try hauto use:subtyping_wf_typ.
+      move : H1 => /(_ _ _ X) H1.
+      simpl in H1. destruct_eq_atom. eapply H1; simpl; eauto.
+      eapply wf_cons_tvar; eauto.
+  - rewrite subst_typ_in_typ_open_typ_wrt_typ.
+    + hauto use:subtyping_wf_typ.
+    + eapply typing_tapp; eauto. fold subst_typ_in_typ.
+      eapply subtyping_subst with (C:=B); eauto.
+Admitted.
+
 Theorem preservation Γ t t' A : 
   uniq Γ ->
   Γ ⊢ t : A ->
